src/tactics/FStar.Tactics.Basic.fsti
@@ -101,3 +101,4 @@ val lset                   : typ -> string -> term -> tac unit
 val curms                  : unit -> tac Z.t
 val set_urgency            : Z.t -> tac unit
 val t_commute_applied_match : unit -> tac unit
+val run_smt                : env -> term -> tac string
