ulib/FStar.Tactics.Builtins.fsti
@@ -362,3 +362,6 @@ val curms : unit -> Tac int
 (** [set_urgency u] sets the urgency of error messages. Usually set just
 before raising an exception (see e.g. [fail_silently]). *)
 val set_urgency : int -> TacS unit
+
+val run_smt: env -> term -> Tac string
+
